proofs/theories/consistency.v
@@ -23,15 +23,13 @@ Fixpoint debruijnDepth a : nat :=
   | tPi _ A B => max (debruijnDepth A) (debruijnDepth B - 1)
   | tSig _ A B => max (debruijnDepth A) (debruijnDepth B - 1)
   | tUniv _ => 0
-  | tEq _ a b A => max (debruijnDepth a) (max (debruijnDepth b) (debruijnDepth A))
+  | tEq _ a b => max (debruijnDepth a) (debruijnDepth b)
   | tRefl => 0
   | tJ _ t p => max (debruijnDepth t - 2) (debruijnDepth p)
-  | tD => 1
   | tVoid => 0
   | tLet _ _ a b => max (debruijnDepth a) (debruijnDepth b - 2)
   | tPack _ a b => max (debruijnDepth a) (debruijnDepth b)
-  | tAbsurd a => debruijnDepth a
-  | tDown _ p => debruijnDepth p
+  | tAbsurd => 0
   end.
 
 Lemma lookup_lt i Γ ℓ A : lookup i Γ ℓ A -> i < length Γ.
@@ -44,9 +42,73 @@ Proof.
   hauto lq:on use:lookup_lt.
 Qed.
 
-Lemma ne_depth_gt0 a : ne a -> debruijnDepth a > 0.
+Fixpoint hasAbsurd a :=
+  match a with
+  | var_tm i => false
+  | tAbs _ b => false
+  | tApp a _ b => hasAbsurd a || hasAbsurd b
+  | tPi _ A B => hasAbsurd A
+  | tSig _ A B => hasAbsurd A
+  | tUniv _ => false
+  | tEq _ a b => hasAbsurd a || hasAbsurd b
+  | tRefl => false
+  | tJ _ t p => hasAbsurd t || hasAbsurd p
+  | tVoid => false
+  | tLet _ _ a b => hasAbsurd a
+  | tPack _ a b => hasAbsurd a || hasAbsurd b
+  | tAbsurd => true
+  end.
+
+Lemma ne_depth_gt0 a : ne a -> debruijnDepth a > 0 \/ hasAbsurd a.
   elim : a => //=; try lia; sfirstorder b:on.
 Qed.
+
+(* Lemma par_absurd_exp a b : a ⇒ b -> hasAbsurd b -> hasAbsurd a. *)
+(* Proof. *)
+(*   move => h. elim : a b /h => //=. *)
+(*   - sfirstorder b:on. *)
+(*   - admit. *)
+(*   - sfirstorder b:on. *)
+(*   - sfirstorder b:on. *)
+(*   - sfirstorder b:on. *)
+(*   - sfirstorder b:on. *)
+(*   - move => _ _ a0 b0 c0 a1 b1 c1 ha iha hb ihb hc ihc. *)
+
+
+
+Lemma ne_ill_type_void ℓ a A : nil ⊢ a ; ℓ ∈ A -> hasAbsurd a -> False.
+  move E : (nil) => Γ h.
+  move : E.
+  elim : Γ ℓ a A /h => //=.
+  - sfirstorder b:on.
+  - move => Γ _ ℓ0 ℓ1 i a A ha iha _ _ ? _. subst.
+    move : ha  =>  /[dup] ha /(proj1 soundness) /(_ nil var_tm ltac:(hauto lq:on use:ρ_ok_id)).
+    move => [m][PA][].
+    asimpl. move /InterpUnivN_Void_inv => -> {PA}[_ [v [hr hv]]].
+    suff : hasAbsurd a by tauto.
+    have hv' : nil ⊢ v ; ℓ0 ∈ tVoid by sfirstorder use:subject_reduction_star.
+    move /wt_dbound in hv'.
+    simpl in hv'.
+    have {}hv' : hasAbsurd v by qauto l:on use:ne_depth_gt0 solve+:lia.
+
+    have : hasAbsurd v by , ne_depth_gt0.
+  - sfirstorder b:on.
+  - sfirstorder b:on.
+
+
+(* Lemma ne_ill_type a ℓ A : nil ⊢ a ; ℓ ∈ A -> ne a \/ A = tVoid -> False. *)
+(* Proof. *)
+  (* move E : nil=> Γ h. *)
+  (* move : E. *)
+  (* elim : Γ ℓ a A / h => //=. *)
+  (* - hauto lq:on inv:lookup. *)
+  (* - sfirstorder. *)
+  (* - sfirstorder. *)
+  (* - best. *)
+  (* - sfirstorder lqb:on. *)
+  (* - move => Γ _ ℓ0 ℓ1 i a A ha iha hA ? ?. subst. *)
+  (*   move /(proj1 soundness) /(_ nil var_tm ltac:(hauto lq:on use:ρ_ok_id)) : ha. *)
+(*   move => [m][PA][]. asimpl. move /InterpUnivN_Void_inv => -> {PA}[_ [v [hr hv]]]. *)
 
 Lemma consistency a ℓ : ~nil ⊢ a ; ℓ ∈ tVoid.
 Proof.
@@ -54,7 +116,11 @@ Proof.
   move => [m][PA][].
   asimpl. move /InterpUnivN_Void_inv => -> {PA}[_ [v [hr hv]]].
   move : subject_reduction_star h hr; repeat move/[apply].
-  move /wt_dbound.
+  move /wt_dbound => //=.
+  move /ne_depth_gt0 : (hv).
+  case => //=. lia.
+
+  case : v hv => //=; try lia.
   move /ne_depth_gt0 : hv => /=. lia.
 Qed.
 
